PolyFun/Realizability/Basic.lean
@@ -5,6 +5,8 @@ Authors: Devon Tuma
 -/
 module
 
+public import PolyFun.Realizability.DynSystem
+public import PolyFun.Realizability.DynSystemClosure
 public import PolyFun.Realizability.Machine
 public import PolyFun.Realizability.StepClass
 
